Swapped the ordering in the List predicates so they are conforming to the norm.

Java/src/CaseStudies/List.v
@@ -4,51 +4,40 @@ Require Import SepAlg SepAlgInsts ILInsts ILogic ILEmbed ILEmbedTac ILQuantTac O
                SepAlgMap UUSepAlg Open Subst Stack Lang SemCmd HeapArr ST SemCmdRules BILogic BILInsts Rel.
 
 Open Scope string_scope.
+Local Existing Instance DecSval.
 
 Fixpoint Node_list (p : val) (xs : list sval) : asn :=
   match xs with
     | nil => embed (p = null)
-    | x :: xs => Exists v, Node_list v xs ** pointsto p "val" x ** pointsto p "next" v 
+    | x :: xs => Exists v, pointsto p "val" x ** pointsto p "next" v ** Node_list v xs  
   end
 .
 
 Definition List_rep (p : val) (xs : list sval) : asn :=
-  Exists head, Node_list head xs ** pointsto p "head" head.
-
-Local Existing Instance DecSval.
+  Exists head, pointsto p "head" head ** Node_list head xs .
 
 Lemma Node_list_decidable (p : val) (xs : list sval) : DecidableAsn (Node_list p xs).
 Proof.
-  generalize dependent p.
-  induction xs.
+  generalize dependent p; induction xs.
   * intros p Pr n h.
     destruct (dec_eq p null); [ left; apply e | right; intro Hfail; auto ].
   * intro p.
-    assert (forall (p' : sval), DecidableAsn (@sepSP asn _ (Node_list p' xs) (pointsto p "val" a))).
-      intros p'. specialize (IHxs p').
-      apply pointsto_decidable_2 with (v := p) (f := "val") (e := a) in IHxs.
-      exact IHxs.
+    assert (forall (p' : sval), DecidableAsn (@sepSP asn _ (Node_list p' xs) (pointsto p "val" a))) by
+      (intros p'; apply pointsto_decidable_2; apply IHxs). 
     apply decidable_existsI with (p := p) (f := "next") in H.
-    unfold Node_list; fold Node_list.
-    setoid_rewrite <- sepSPA.
-    exact H.
+    setoid_rewrite sepSPA in H; setoid_rewrite <- sepSPC in H; setoid_rewrite sepSPA in H.
+    apply H.
 Qed.
 
 Lemma List_rep_decidable (p : val) (xs : list sval) : DecidableAsn (List_rep p xs).
-Proof.  
-  unfold List_rep.
+Proof.
+  unfold List_rep; setoid_rewrite sepSPC.
   apply decidable_existsI.
   intro p'; apply Node_list_decidable.
 Qed.
 
 Lemma List_rep_decidable_val (p : val) (xs : list sval) : DecidableSasn (`List_rep `p `xs).
-Proof.
-  intros s. unfold liftn, lift; simpl.
-  apply List_rep_decidable.
-Qed.
+Proof. intros s; unfold liftn, lift; simpl; apply List_rep_decidable. Qed.
 
 Lemma List_rep_decidable_var (p : var) (xs : list sval) : DecidableSasn (`List_rep p/V `xs).
-Proof.
-  intros s. unfold liftn, lift, var_expr; simpl.
-  apply List_rep_decidable.
-Qed.
+Proof. intros s; unfold liftn, lift, var_expr; simpl; apply List_rep_decidable. Qed.
